Multiplication on ℕ distributes over addition

Lean4Axiomatic/AbstractAlgebra.lean
@@ -139,6 +139,98 @@ def cancelR_from_cancelL
   have : rβ (f x y₁) (f x y₂) := AA.substR (rβ := (· → ·)) AA.comm this
   exact AA.cancelL this
 
+/--
+Class for types and operations that satisfy either the left- or right-handed
+distributive property.
+
+For more information see `DistributiveOn.distrib` or
+[consult Wikipedia](https://en.wikipedia.org/wiki/Distributive_property).
+
+**Named parameters**
+- `hand`: indicates whether the property is left- or right-handed.
+- `α`: the type that the binary operations `f` and `g` are defined over.
+- `f`: the binary operation that distributes over `g`.
+- `g`: the binary operation that `f` distributes over.
+
+**Class parameters**
+- `EqvOp α`: necessary because the property expresses an equality on `α`.
+-/
+class DistributiveOn
+    (hand : Hand) {α : Sort u} [EqvOp α] (f g : α → α → α) where
+  /--
+  The left- or right-handed distributive property of two binary operations `f`
+  and `g` defined over a type `α`.
+
+  If this property is satisfied, one says that `f` _distributes_ over `g`. A
+  well-known example from arithmetic is that multiplication distributes over
+  addition; `a * (b + c) ≃ a * b + a * c` for the left-handed case and
+  `(b + c) * a ≃ b * a + c * a` for the right-handed case.
+
+  **Named parameters**
+  - see `DistributiveOn` for the class parameters.
+  - `x`: the argument to `f` that gets distributed; the `hand` parameter
+    indicates which side of `f` it is on.
+  - `y`: the left argument to `g`.
+  - `z`: the right argument to `g`.
+  -/
+  distrib {x y z : α} :
+    let f' := forHand hand f
+    f' x (g y z) ≃ g (f' x y) (f' x z)
+
+export DistributiveOn (distrib)
+
+/--
+Convenience function for the left-handed distributive property.
+
+Can often resolve cases where type inference gets stuck when using the more
+general `distrib` function.
+
+See `DistributiveOn.distrib` for detailed documentation.
+-/
+abbrev distribL := @distrib Hand.L
+
+/--
+Convenience function for the right-handed distributive property.
+
+Can often resolve cases where type inference gets stuck when using the more
+general `distrib` function.
+
+See `DistributiveOn.distrib` for detailed documentation.
+-/
+abbrev distribR := @distrib Hand.R
+
+/--
+Convenience class for types and operations that satisfy the full (left- **and**
+right-handed) distributive property.
+
+See `DistributiveOn` for detailed documentation.
+-/
+class Distributive {α : Sort u} [EqvOp α] (f g : α → α → α) where
+  distributiveL : DistributiveOn Hand.L f g
+  distributiveR : DistributiveOn Hand.R f g
+
+attribute [instance] Distributive.distributiveL
+attribute [instance] Distributive.distributiveR
+
+/--
+Derive right-distributivity from left-distributivity for operations `f` and `g`
+meeting certain conditions.
+-/
+def distributiveR_from_distributiveL
+    {α : Sort u} {f g : α → α → α}
+    [EqvOp α] [Commutative f] [Substitutive₂ g (· ≃ ·) (· ≃ ·)]
+    : DistributiveOn Hand.L f g → DistributiveOn Hand.R f g := by
+  intro
+  constructor
+  intro x y z f'
+  show f (g y z) x ≃ g (f y x) (f z x)
+  calc
+    f (g y z) x       ≃ _ := AA.comm
+    f x (g y z)       ≃ _ := AA.distribL
+    g (f x y) (f x z) ≃ _ := AA.substL AA.comm
+    g (f y x) (f x z) ≃ _ := AA.substR AA.comm
+    g (f y x) (f z x) ≃ _ := Eqv.refl
+
 inductive OneOfThree (α β γ : Prop) : Prop where
 | first  (a : α)
 | second (b : β)
